contrib/setoid_ring/Field_tac.v
@@ -70,7 +70,7 @@ Ltac FFV Cst CstPow add mul sub opp div inv pow t fv :=
 Ltac ParseFieldComponents lemma req :=
   match type of lemma with
   | context [
-        PCond _ _ _  _ _ _ _  _ _  _ _ ->
+     (*   PCond _ _ _  _ _ _ _  _ _  _ _ -> *)
         req (@FEeval ?R ?rO ?radd ?rmul ?rsub ?ropp ?rdiv ?rinv 
                           ?C ?phi ?Cpow ?Cp_phi ?rpow _ _) _ ] =>
       (fun f => f radd rmul rsub ropp rdiv rinv rpow C)
@@ -93,7 +93,11 @@ Ltac fold_field_cond req :=
 
 Ltac simpl_PCond req :=
   protect_fv "field_cond";
-  try (exact I);
+  (try exact I);
+  fold_field_cond req.
+
+Ltac simpl_PCond_BEURK req :=
+  protect_fv "field_cond";
   fold_field_cond req.
 
 (* Rewriting (field_simplify) *)
@@ -129,32 +133,60 @@ Ltac Field_norm_gen f Cst_tac Pow_tac lemma Cond_lemma req n lH rl :=
   ParseFieldComponents lemma req Main.
 
 Ltac Field_simplify_gen f := 
-     fun req cst_tac pow_tac _ _ field_simplify_ok cond_ok pre post lH rl =>
+     fun req cst_tac pow_tac _ _ field_simplify_ok _ cond_ok pre post lH rl =>
        pre(); 
        Field_norm_gen f cst_tac pow_tac field_simplify_ok cond_ok req 
                   ring_subst_niter lH rl; 
       post().
 
 Ltac Field_simplify := Field_simplify_gen ltac:(fun H => rewrite H).
+
+Tactic Notation (at level 0) 
+  "field_simplify" constr_list(rl) :=
+  match goal with [|- ?G] => field_lookup Field_simplify [] rl [G] end.
+
+Tactic Notation (at level 0) 
+  "field_simplify" "[" constr_list(lH) "]" constr_list(rl) :=
+  match goal with [|- ?G] => field_lookup Field_simplify [lH] rl [G] end.
+
+Tactic Notation "field_simplify" constr_list(rl) "in" hyp(H):=   
+ match goal with 
+ | [|- ?G] =>
+   let t := type of H in   
+   let g := fresh "goal" in
+   set (g:= G);
+   generalize H;clear H;
+   field_lookup Field_simplify [] rl [t];
+   intro H;
+   unfold g;clear g
+ end.
+
+Tactic Notation "field_simplify" "["constr_list(lH) "]" constr_list(rl) "in" hyp(H):=   
+ match goal with 
+ | [|- ?G] =>
+   let t := type of H in   
+   let g := fresh "goal" in
+   set (g:= G);
+   generalize H;clear H;
+   field_lookup Field_simplify [lH] rl [t];
+   intro H;
+   unfold g;clear g
+ end.
+
+(*
 Ltac Field_simplify_in hyp:= 
    Field_simplify_gen ltac:(fun H => rewrite H in hyp).
 
 Tactic Notation (at level 0) 
-  "field_simplify" constr_list(rl) :=
-  field_lookup Field_simplify [] rl.
-
-Tactic Notation (at level 0) 
-  "field_simplify" "[" constr_list(lH) "]" constr_list(rl) :=
-  field_lookup Field_simplify [lH] rl.
-
-Tactic Notation (at level 0) 
   "field_simplify" constr_list(rl) "in" hyp(h) :=
-  field_lookup (Field_simplify_in h) [] rl.
+  let t := type of h in
+  field_lookup (Field_simplify_in h) [] rl [t].
 
 Tactic Notation (at level 0) 
   "field_simplify" "[" constr_list(lH) "]" constr_list(rl) "in" hyp(h) :=
-  field_lookup (Field_simplify_in h) [lH] rl.
-
+  let t := type of h in
+  field_lookup (Field_simplify_in h) [lH] rl [t].
+*)
 
 (** Generic tactic for solving equations *)
 
@@ -193,7 +225,8 @@ Ltac Field_Scheme Simpl_tac Cst_tac Pow_tac lemma Cond_lemma req n lH :=
          ltac:(fun ilemma =>
                   apply ilemma 
                   || fail "field anomaly: failed in applying lemma";
-                  [ Simpl_tac | apply Cond_lemma; simpl_PCond req]) in
+                  [ Simpl_tac | apply Cond_lemma; simpl_PCond req]);
+      clear vlpe nlemma in
     OnEquation req Main_eq in
   ParseFieldComponents lemma req Main.
 
@@ -202,34 +235,105 @@ Ltac Field_Scheme Simpl_tac Cst_tac Pow_tac lemma Cond_lemma req n lH :=
 
 Ltac FIELD :=
    let Simpl := vm_compute; reflexivity || fail "not a valid field equation" in
-   fun req cst_tac pow_tac field_ok _ _ cond_ok pre post lH rl =>
+   fun req cst_tac pow_tac field_ok _ _ _ cond_ok pre post lH rl =>
        pre(); 
        Field_Scheme Simpl cst_tac pow_tac field_ok cond_ok req 
-         Ring_tac.ring_subst_niter lH; 
+         Ring_tac.ring_subst_niter lH;
+       try exact I;
        post().
  
 Tactic Notation (at level 0) "field" :=
-  field_lookup FIELD [].
+  match goal with [|- ?G] => field_lookup FIELD [] [G] end.
 
 Tactic Notation (at level 0) "field" "[" constr_list(lH) "]" :=
-  field_lookup FIELD [lH].
+  match goal with [|- ?G] => field_lookup FIELD [lH] [G] end.
 
 (* transforms a field equation to an equivalent (simplified) ring equation,
    and leaves non-zero conditions to be proved (field_simplify_eq) *)
 Ltac FIELD_SIMPL  :=
   let Simpl := (protect_fv "field") in
-  fun req cst_tac pow_tac _ field_simplify_eq_ok _ cond_ok pre post lH rl =>
+  fun req cst_tac pow_tac _ field_simplify_eq_ok _ _ cond_ok pre post lH rl =>
        pre(); 
        Field_Scheme Simpl cst_tac pow_tac field_simplify_eq_ok cond_ok 
           req Ring_tac.ring_subst_niter lH;
        post().
 
 Tactic Notation (at level 0) "field_simplify_eq" :=  
-  field_lookup FIELD_SIMPL [].
+  match goal with [|- ?G] => field_lookup FIELD_SIMPL [] [G] end.
 
 Tactic Notation (at level 0) "field_simplify_eq" "[" constr_list(lH) "]" :=  
-  field_lookup FIELD_SIMPL [lH].
+  match goal with [|- ?G] => field_lookup FIELD_SIMPL [lH] [G] end.
 
+(* Same as FIELD_SIMPL but in hypothesis *)
+
+Ltac Field_simplify_eq Cst_tac Pow_tac lemma Cond_lemma req n lH :=
+   let Main radd rmul rsub ropp rdiv rinv rpow C :=
+    let hyp := fresh "hyp" in
+    intro hyp;
+    match type of hyp with
+    | req ?t1 ?t2 =>
+      let mkFV := FV Cst_tac Pow_tac radd rmul rsub ropp rpow in
+      let mkPol := mkPolexpr C Cst_tac Pow_tac radd rmul rsub ropp rpow in
+      let mkFFV := FFV Cst_tac Pow_tac radd rmul rsub ropp rdiv rinv rpow in
+      let mkFE := 
+        mkFieldexpr C Cst_tac Pow_tac radd rmul rsub ropp rdiv rinv rpow in
+      let rec ParseExpr ilemma :=
+        match type of ilemma with
+        |  forall nfe, ?fe = nfe -> _ =>
+          (fun t => 
+            let x := fresh "fld_expr" in 
+            let H := fresh "norm_fld_expr" in
+            compute_assertion H x fe;
+            ParseExpr (ilemma x H) t;
+            try clear H x)
+        | _ => (fun t => t ilemma)
+        end in
+      let fv := FV_hypo_tac mkFV req lH in
+      let fv := mkFFV t1 fv in
+      let fv := mkFFV t2 fv in
+      let lpe := mkHyp_tac C req ltac:(fun t => mkPol t fv) lH in
+      let prh := proofHyp_tac lH in
+      let fe1 := mkFE t1 fv in
+      let fe2 := mkFE t2 fv in
+      let vlpe := fresh "vlpe" in
+      ParseExpr (lemma n fv lpe fe1 fe2 prh)
+         ltac:(fun ilemma =>
+             match type of ilemma with
+             | req _ _ ->  _ -> ?EQ => 
+               let tmp := fresh "tmp" in
+               assert (tmp : EQ);
+               [ apply ilemma; 
+                 [ exact hyp | apply Cond_lemma; simpl_PCond_BEURK req]
+               | protect_fv "field" in tmp;
+                 generalize tmp;clear tmp ];
+               clear hyp  
+             end)
+     end in
+  ParseFieldComponents lemma req Main.
+
+Ltac FIELD_SIMPL_EQ :=
+ fun req cst_tac pow_tac _ _ _ lemma cond_ok pre post lH rl =>
+       pre(); 
+       Field_simplify_eq cst_tac pow_tac lemma cond_ok req
+         Ring_tac.ring_subst_niter lH;
+       post().
+
+Tactic Notation (at level 0) "field_simplify_eq" "in" hyp(H) :=
+  let t := type of H in
+  generalize H;
+  field_lookup FIELD_SIMPL_EQ [] [t];
+  [ try exact I
+  | clear H;intro H].
+
+
+Tactic Notation (at level 0) 
+  "field_simplify_eq" "[" constr_list(lH) "]"  "in" hyp(H) :=  
+  let t := type of H in
+  generalize H;
+  field_lookup FIELD_SIMPL_EQ [lH] [t];
+  [ try exact I
+  |clear H;intro H].
+ 
 (* Adding a new field *)
 
 Ltac ring_of_field f :=
@@ -258,6 +362,11 @@ Ltac field_lemmas set ext inv_m fspec pspec sspec rk :=
      | None => constr:(Field_simplify_eq_correct)
      | Some _ => constr:(Field_simplify_eq_pow_correct)
      end in
+  let simpl_eq_in_lemma :=
+     match pspec with
+     | None => constr:(Field_simplify_eq_in_correct)
+     | Some _ => constr:(Field_simplify_eq_pow_in_correct)
+     end in
   let rw_lemma :=
      match pspec with
      | None => constr:(Field_rw_correct)
@@ -278,6 +387,11 @@ Ltac field_lemmas set ext inv_m fspec pspec sspec rk :=
                    set ext_r inv_m afth 
                    _ _ _  _ _ _  _ _ _ morph 
                    _ _ _ pp_spec _ ss_spec) in
+       let field_simpl_eq_in :=
+         constr:(simpl_eq_in_lemma _ _ _  _ _ _  _ _ _ _
+                   set ext_r inv_m afth 
+                   _ _ _  _ _ _  _ _ _ morph 
+                   _ _ _ pp_spec _ ss_spec) in
        let field_ok := 
          constr:(Field_correct set ext_r inv_m afth morph pp_spec ss_spec) in
        let cond1_ok := 
@@ -285,9 +399,10 @@ Ltac field_lemmas set ext inv_m fspec pspec sspec rk :=
        let cond2_ok := 
          constr:(Pcond_simpl_complete set ext_r afth morph pp_spec) in
        (fun f => 
-         f afth ext_r morph field_ok field_simpl_ok field_simpl_eq_ok
+         f afth ext_r morph field_ok field_simpl_ok field_simpl_eq_ok field_simpl_eq_in
                 cond1_ok cond2_ok)
      | _ => fail 2 "bad sign specification"
      end 
      | _ => fail 1 "bad power specification" 
      end).
+
